[sledge sem] Refactor the way LLVM sem. does phis
Summary:
Previously the LLVM semantics did the phi instructions at the head of a
block as part of executing the branch into that block. This looked a bit
weird, but had the advantage that the semantics knew which block was
being jumped from, which is necessary to run the phi instructions.
However, it meant that the rules for doing phi instructions would need
to show up with each branching construct. It was also annoying for the
LLVM->llair proof, since the phis are removed and their effect happens as
a distinct step from the branch.

Here we add a distinct Phi_ip instruction pointer to indicate that the
phi instructions at the start of the block should execute next, and then
be incremented to the usual numeric instruction pointer that points to
the non-phi instructions. The Phi_ip contains the identity of the
previous block.

Reviewed By: jberdine

Differential Revision: D17452416

fbshipit-source-id: 78fef7cca

sledge/semantics/llvmScript.sml
@@ -69,6 +69,21 @@ Datatype:
 End
 
 Datatype:
+  phi = Phi reg ty ((label option, arg) alist)
+End
+
+(*
+ * The Exit instruction below models a system/libc call to exit the program. The
+ * semantics needs some way to tell the difference between normally terminated
+ * programs and stuck states, and this lets it do that. From a C++ perspective,
+ * a program could call this directly, in which case it's good to model, or it
+ * might simply return from main and then the code in libc that called main will
+ * call exit. However, adding special handling for main in the semantics will
+ * cruft things up a bit, and it's not very satisfying, because it's not really
+ * an LLVM concept.
+ *)
+
+Datatype:
   instr =
   (* Terminators *)
   | Ret targ
@@ -94,10 +109,6 @@ Datatype:
   | Cxa_begin_catch reg arg
   | Cxa_end_catch
   | Cxa_get_exception_ptr reg arg
-End
-
-Datatype:
-  phi = Phi reg ty ((label option, arg) alist)
 End
 
 Datatype:
@@ -160,8 +171,17 @@ Datatype:
   pv = <| poison : bool; value : v |>
 End
 
+(* Instruction pointer into a block. Phi_ip indicates to do the phi instruction,
+ * coming from the given label. Offset points to a normal (non-phi) instruction.
+ * *)
 Datatype:
-  pc = <| f : fun_name; b : label option; i : num |>
+  bip =
+  | Phi_ip (label option)
+  | Offset num
+End
+
+Datatype:
+  pc = <| f : fun_name; b : label option; i : bip |>
 End
 
 Datatype:
@@ -461,8 +481,13 @@ Definition update_result_def:
   update_result x v s = s with locals := s.locals |+ (x, v)
 End
 
+Definition inc_bip_def:
+  (inc_bip (Phi_ip _) = Offset 0) ∧
+  (inc_bip (Offset i) = Offset (i + 1))
+End
+
 Definition inc_pc_def:
-  inc_pc s = s with ip := (s.ip with i := s.ip.i + 1)
+  inc_pc s = s with ip := (s.ip with i := inc_bip s.ip.i)
 End
 
 Inductive get_obs:
@@ -488,27 +513,12 @@ Inductive step_instr:
           stack := st;
           heap := new_h |>)) ∧
 
-(* Do the phi assignments in parallel. The manual says "For the purposes of the
- * SSA form, the use of each incoming value is deemed to occur on the edge from
- * the corresponding predecessor block to the current block (but after any
- * definition of an 'invoke' instruction's return value on the same edge)".
- * So treat these two as equivalent
- * %r1 = phi [0, %l]
- * %r2 = phi [%r1, %l]
- * and
- * %r2 = phi [%r1, %l]
- * %r1 = phi [0, %l]
- *)
   (eval s a = Some <| poison := p; value := FlatV (W1V tf) |> ∧
-   l = Some (if tf = 1w then l1 else l2) ∧
-   alookup prog s.ip.f = Some d ∧
-   alookup d.blocks l = Some <| h := Head phis None; body := b |> ∧
-   map (do_phi l s) phis = map Some updates
+   l = Some (if tf = 1w then l1 else l2)
    ⇒
    step_instr prog s
      (Br a l1 l2) Tau
-     (s with <| ip := <| f := s.ip.f; b := l; i := 0 |>;
-                locals := s.locals |++ updates |>)) ∧
+     (s with ip := <| f := s.ip.f; b := l; i := Phi_ip s.ip.b |>)) ∧
 
   (* TODO *)
   (step_instr prog s (Invoke r t a args l1 l2) Tau s) ∧
@@ -623,11 +633,12 @@ Inductive step_instr:
    ⇒
    step_instr prog s
      (Call r t fname targs) Tau
-     <| ip := <| f := fname; b := None; i := 0 |>;
+     (* Jump to the entry block of the function which has no phis *)
+     <| ip := <| f := fname; b := None; i := Offset 0 |>;
         locals := alist_to_fmap (zip (map snd d.params, vs));
         globals := s.globals;
         stack :=
-          <| ret := s.ip with i := s.ip.i + 1;
+          <| ret := s.ip with i := inc_bip s.ip.i;
              saved_locals := s.locals;
              result_var := r;
              stack_allocs := [] |> :: s.stack;
@@ -647,24 +658,49 @@ Inductive step_instr:
 End
 
 Inductive get_instr:
-  (∀prog ip.
-   alookup prog ip.f = Some d ∧
-   alookup d.blocks ip.b = Some b ∧
-   ip.i < length b.body
-   ⇒
-   get_instr prog ip (el ip.i b.body))
+ (∀prog ip.
+  alookup prog ip.f = Some d ∧
+  alookup d.blocks ip.b = Some b ∧
+  ip.i = Offset idx ∧
+  idx < length b.body
+  ⇒
+  get_instr prog ip (Inl (el idx b.body))) ∧
+ (∀prog ip.
+  alookup prog ip.f = Some d ∧
+  alookup d.blocks ip.b = Some b ∧
+  ip.i = Phi_ip from_l ∧
+  b.h = Head phis landing
+  ⇒
+  get_instr prog ip (Inr (from_l, phis)))
 End
 
 Inductive step:
-  get_instr p s.ip i ∧
+ (get_instr p s.ip (Inl i) ∧
   step_instr p s i l s'
   ⇒
-  step p s l s'
+  step p s l s') ∧
+
+(* Do the phi assignments in parallel. The manual says "For the purposes of the
+ * SSA form, the use of each incoming value is deemed to occur on the edge from
+ * the corresponding predecessor block to the current block (but after any
+ * definition of an 'invoke' instruction's return value on the same edge)".
+ * So treat these two as equivalent
+ * %r1 = phi [0, %l]
+ * %r2 = phi [%r1, %l]
+ * and
+ * %r2 = phi [%r1, %l]
+ * %r1 = phi [0, %l]
+ *)
+ (get_instr p s.ip (Inr (from_l, phis)) ∧
+  map (do_phi from_l s) phis = map Some updates
+  ⇒
+  step p s Tau (inc_pc (s with locals := locals |++ updates)))
+
 End
 
 Definition get_observation_def:
   get_observation prog last_s =
-    if get_instr prog last_s.ip Exit then
+    if get_instr prog last_s.ip (Inl Exit) then
       Complete
     else if ∃s l. step prog last_s l s then
       Partial
@@ -695,20 +731,39 @@ End
 (* Instruction pointer points to an instruction *)
 Definition ip_ok_def:
   ip_ok p ip ⇔
-    ∃dec block. alookup p ip.f = Some dec ∧ alookup dec.blocks ip.b = Some block ∧ ip.i < length block.body
+    ∃dec block.
+      alookup p ip.f = Some dec ∧ alookup dec.blocks ip.b = Some block ∧
+      ((∃idx. ip.i = Offset idx ∧ idx < length block.body) ∨
+       (∃from_l. ip.i = Phi_ip from_l ∧ block.h ≠ Entry ∧ alookup dec.blocks from_l ≠ None))
+End
+
+Definition instr_to_labs_def:
+  (instr_to_labs (Br _ l1 l2) = [l1; l2]) ∧
+  (instr_to_labs _ = [])
 End
 
 Definition prog_ok_def:
   prog_ok p ⇔
-    ((* All blocks end with terminators *)
+    ((* All blocks end with terminators and terminators only appear at the end.
+      * All labels mentioned in instructions actually exist *)
      ∀fname dec bname block.
        alookup p fname = Some dec ∧
        alookup dec.blocks bname = Some block
        ⇒
-       block.body ≠ [] ∧ terminator (last block.body)) ∧
+       block.body ≠ [] ∧ terminator (last block.body) ∧
+       every (λi. ¬terminator i) (front block.body) ∧
+       every (λlab. alookup dec.blocks (Some lab) ≠ None)
+             (instr_to_labs (last block.body)) ∧
+       (∀phis lands. block.h = Head phis lands ⇒
+         every (λx. case x of Phi _ _ l => every (λ(lab, _). alookup dec.blocks lab ≠ None) l) phis)) ∧
     ((* All functions have an entry block *)
      ∀fname dec.
-       alookup p fname = Some dec ⇒ ∃block. alookup dec.blocks None = Some block) ∧
+       alookup p fname = Some dec ⇒
+       ∃block. alookup dec.blocks None = Some block ∧ block.h = Entry) ∧
+    ((* All non-entry blocks have a proper header *)
+     ∀fname dec l b.
+       alookup p fname = Some dec ∧ alookup dec.blocks (Some l) = Some b ⇒
+       b.h ≠ Entry) ∧
      (* There is a main function *)
      ∃dec. alookup p (Fn "main") = Some dec
 End
@@ -740,7 +795,7 @@ Definition is_init_state_def:
   is_init_state s (global_init : glob_var |-> ty # v) ⇔
     s.ip.f = Fn "main" ∧
     s.ip.b = None ∧
-    s.ip.i = 0 ∧
+    s.ip.i = Offset 0 ∧
     s.locals = fempty ∧
     s.stack = [] ∧
     globals_ok s ∧
