sledge/semantics/llvm_liveScript.sml
@@ -16,35 +16,47 @@ new_theory "llvm_live";
 numLib.prefer_num ();
 
 Definition inc_pc_def:
-  inc_pc ip = ip with i := ip.i + 1
+  inc_pc ip = ip with i := inc_bip ip.i
 End
 
 (* The set of program counters the given instruction and starting point can
  * immediately reach, within a function *)
-Definition next_ips_def:
-  (next_ips (Ret _) ip = {}) ∧
-  (next_ips (Br _ l1 l2) ip =
-    { <| f := ip.f; b := Some l; i := 0 |> | l | l ∈ {l1; l2} }) ∧
-  (next_ips (Invoke _ _ _ _ l1 l2) ip =
-    { <| f := ip.f; b := Some l; i := 0 |> | l | l ∈ {l1; l2} }) ∧
-  (next_ips Unreachable ip = {}) ∧
-  (next_ips (Sub _ _ _ _ _ _) ip = { inc_pc ip }) ∧
-  (next_ips (Extractvalue _ _ _) ip = { inc_pc ip }) ∧
-  (next_ips (Insertvalue _ _ _ _) ip = { inc_pc ip }) ∧
-  (next_ips (Alloca _ _ _) ip = { inc_pc ip }) ∧
-  (next_ips (Load _ _ _) ip = { inc_pc ip }) ∧
-  (next_ips (Store _ _) ip = { inc_pc ip }) ∧
-  (next_ips (Gep _ _ _ _) ip = { inc_pc ip }) ∧
-  (next_ips (Ptrtoint _ _ _) ip = { inc_pc ip }) ∧
-  (next_ips (Inttoptr _ _ _) ip = { inc_pc ip }) ∧
-  (next_ips (Icmp _ _ _ _ _) ip = { inc_pc ip }) ∧
-  (next_ips (Call _ _ _ _) ip = { inc_pc ip }) ∧
-  (next_ips (Cxa_allocate_exn _ _) ip = { inc_pc ip }) ∧
+Definition instr_next_ips_def:
+  (instr_next_ips (Ret _) ip = {}) ∧
+  (instr_next_ips (Br _ l1 l2) ip =
+    { <| f := ip.f; b := Some l; i := Phi_ip ip.b |> | l | l ∈ {l1; l2} }) ∧
+  (instr_next_ips (Invoke _ _ _ _ l1 l2) ip =
+    { <| f := ip.f; b := Some l; i := Phi_ip ip.b |> | l | l ∈ {l1; l2} }) ∧
+  (instr_next_ips Unreachable ip = {}) ∧
+  (instr_next_ips (Sub _ _ _ _ _ _) ip = { inc_pc ip }) ∧
+  (instr_next_ips (Extractvalue _ _ _) ip = { inc_pc ip }) ∧
+  (instr_next_ips (Insertvalue _ _ _ _) ip = { inc_pc ip }) ∧
+  (instr_next_ips (Alloca _ _ _) ip = { inc_pc ip }) ∧
+  (instr_next_ips (Load _ _ _) ip = { inc_pc ip }) ∧
+  (instr_next_ips (Store _ _) ip = { inc_pc ip }) ∧
+  (instr_next_ips (Gep _ _ _ _) ip = { inc_pc ip }) ∧
+  (instr_next_ips (Ptrtoint _ _ _) ip = { inc_pc ip }) ∧
+  (instr_next_ips (Inttoptr _ _ _) ip = { inc_pc ip }) ∧
+  (instr_next_ips (Icmp _ _ _ _ _) ip = { inc_pc ip }) ∧
+  (instr_next_ips (Call _ _ _ _) ip = { inc_pc ip }) ∧
+  (instr_next_ips (Cxa_allocate_exn _ _) ip = { inc_pc ip }) ∧
   (* TODO: revisit throw when dealing with exceptions *)
-  (next_ips (Cxa_throw _ _ _) ip = {  }) ∧
-  (next_ips (Cxa_begin_catch _ _) ip = { inc_pc ip }) ∧
-  (next_ips (Cxa_end_catch) ip = { inc_pc ip }) ∧
-  (next_ips (Cxa_get_exception_ptr _ _) ip = { inc_pc ip })
+  (instr_next_ips (Cxa_throw _ _ _) ip = {  }) ∧
+  (instr_next_ips (Cxa_begin_catch _ _) ip = { inc_pc ip }) ∧
+  (instr_next_ips (Cxa_end_catch) ip = { inc_pc ip }) ∧
+  (instr_next_ips (Cxa_get_exception_ptr _ _) ip = { inc_pc ip })
+End
+
+Inductive next_ips:
+ (∀prog ip i l.
+    get_instr prog ip (Inl i) ∧
+    l ∈ instr_next_ips i ip
+    ⇒
+    next_ips prog ip l) ∧
+ (∀prog ip from_l phis.
+    get_instr prog ip (Inr (from_l, phis))
+    ⇒
+    next_ips prog ip (inc_pc ip))
 End
 
 (* The path is a list of program counters that represent a statically feasible
@@ -52,14 +64,13 @@ End
 Inductive good_path:
   (∀prog. good_path prog []) ∧
 
-  (∀ip i.
+  (∀prog ip i.
     get_instr prog ip i
     ⇒
     good_path prog [ip]) ∧
 
-  (∀prog path ip1 i1 ip2.
-    get_instr prog ip1 i1 ∧
-    ip2 ∈ next_ips i1 ip1 ∧
+  (∀prog path ip1 ip2.
+    ip2 ∈ next_ips prog ip1 ∧
     good_path prog (ip2::path)
     ⇒
     good_path prog (ip1::ip2::path))
@@ -71,65 +82,102 @@ Definition arg_to_regs_def:
 End
 
 (* The registers that an instruction uses *)
-Definition uses_def:
-  (uses (Ret (_, a)) = arg_to_regs a) ∧
-  (uses (Br a _ _) = arg_to_regs a) ∧
-  (uses (Invoke _ _ a targs _ _) =
+Definition instr_uses_def:
+  (instr_uses (Ret (_, a)) = arg_to_regs a) ∧
+  (instr_uses (Br a _ _) = arg_to_regs a) ∧
+  (instr_uses (Invoke _ _ a targs _ _) =
     arg_to_regs a ∪ BIGUNION (set (map (arg_to_regs o snd) targs))) ∧
-  (uses Unreachable = {}) ∧
-  (uses (Sub _ _ _ _ a1 a2) =
+  (instr_uses Unreachable = {}) ∧
+  (instr_uses (Sub _ _ _ _ a1 a2) =
     arg_to_regs a1 ∪ arg_to_regs a2) ∧
-  (uses (Extractvalue _ (_, a) _) = arg_to_regs a) ∧
-  (uses (Insertvalue _ (_, a1) (_, a2) _) =
+  (instr_uses (Extractvalue _ (_, a) _) = arg_to_regs a) ∧
+  (instr_uses (Insertvalue _ (_, a1) (_, a2) _) =
     arg_to_regs a1 ∪ arg_to_regs a2) ∧
-  (uses (Alloca _ _ (_, a)) = arg_to_regs a) ∧
-  (uses (Load _ _ (_, a)) = arg_to_regs a) ∧
-  (uses (Store (_, a1) (_, a2)) =
+  (instr_uses (Alloca _ _ (_, a)) = arg_to_regs a) ∧
+  (instr_uses (Load _ _ (_, a)) = arg_to_regs a) ∧
+  (instr_uses (Store (_, a1) (_, a2)) =
     arg_to_regs a1 ∪ arg_to_regs a2) ∧
-  (uses (Gep _ _ (_, a) targs) =
+  (instr_uses (Gep _ _ (_, a) targs) =
     arg_to_regs a ∪ BIGUNION (set (map (arg_to_regs o snd) targs))) ∧
-  (uses (Ptrtoint _ (_, a) _) = arg_to_regs a) ∧
-  (uses (Inttoptr _ (_, a) _) = arg_to_regs a) ∧
-  (uses (Icmp _ _ _ a1 a2) =
+  (instr_uses (Ptrtoint _ (_, a) _) = arg_to_regs a) ∧
+  (instr_uses (Inttoptr _ (_, a) _) = arg_to_regs a) ∧
+  (instr_uses (Icmp _ _ _ a1 a2) =
     arg_to_regs a1 ∪ arg_to_regs a2) ∧
-  (uses (Call _ _ _ targs) =
+  (instr_uses (Call _ _ _ targs) =
     BIGUNION (set (map (arg_to_regs o snd) targs))) ∧
-  (uses (Cxa_allocate_exn _ a) = arg_to_regs a) ∧
-  (uses (Cxa_throw a1 a2 a3) =
+  (instr_uses (Cxa_allocate_exn _ a) = arg_to_regs a) ∧
+  (instr_uses (Cxa_throw a1 a2 a3) =
     arg_to_regs a1 ∪ arg_to_regs a2 ∪ arg_to_regs a3) ∧
-  (uses (Cxa_begin_catch _ a) = arg_to_regs a) ∧
-  (uses (Cxa_end_catch) = {  }) ∧
-  (uses (Cxa_get_exception_ptr _ a) = arg_to_regs a)
+  (instr_uses (Cxa_begin_catch _ a) = arg_to_regs a) ∧
+  (instr_uses (Cxa_end_catch) = {  }) ∧
+  (instr_uses (Cxa_get_exception_ptr _ a) = arg_to_regs a)
+End
+
+Definition phi_uses_def:
+  phi_uses from_l (Phi _ _ entries) =
+    case alookup entries from_l of
+    | None => {}
+    | Some a => arg_to_regs a
+End
+
+Inductive uses:
+ (∀prog ip i r.
+    get_instr prog ip (Inl i) ∧
+    r ∈ instr_uses i
+    ⇒
+    uses prog ip r) ∧
+ (∀prog ip from_l phis r.
+   get_instr prog ip (Inr (from_l, phis)) ∧
+    r ∈ BIGUNION (set (map (phi_uses from_l) phis))
+    ⇒
+    uses prog ip r)
 End
 
 (* The registers that an instruction assigns *)
-Definition assigns_def:
-  (assigns (Invoke r _ _ _ _ _) = {r}) ∧
-  (assigns (Sub r _ _ _ _ _) = {r}) ∧
-  (assigns (Extractvalue r _ _) = {r}) ∧
-  (assigns (Insertvalue r _ _ _) = {r}) ∧
-  (assigns (Alloca r _ _) = {r}) ∧
-  (assigns (Load r _ _) = {r}) ∧
-  (assigns (Gep r _ _ _) = {r}) ∧
-  (assigns (Ptrtoint r _ _) = {r}) ∧
-  (assigns (Inttoptr r _ _) = {r}) ∧
-  (assigns (Icmp r _ _ _ _) = {r}) ∧
-  (assigns (Call r _ _ _) = {r}) ∧
-  (assigns (Cxa_allocate_exn r _) = {r}) ∧
-  (assigns (Cxa_begin_catch r _) = {r}) ∧
-  (assigns (Cxa_get_exception_ptr r _) = {r}) ∧
-  (assigns _ = {})
+Definition instr_assigns_def:
+  (instr_assigns (Invoke r _ _ _ _ _) = {r}) ∧
+  (instr_assigns (Sub r _ _ _ _ _) = {r}) ∧
+  (instr_assigns (Extractvalue r _ _) = {r}) ∧
+  (instr_assigns (Insertvalue r _ _ _) = {r}) ∧
+  (instr_assigns (Alloca r _ _) = {r}) ∧
+  (instr_assigns (Load r _ _) = {r}) ∧
+  (instr_assigns (Gep r _ _ _) = {r}) ∧
+  (instr_assigns (Ptrtoint r _ _) = {r}) ∧
+  (instr_assigns (Inttoptr r _ _) = {r}) ∧
+  (instr_assigns (Icmp r _ _ _ _) = {r}) ∧
+  (instr_assigns (Call r _ _ _) = {r}) ∧
+  (instr_assigns (Cxa_allocate_exn r _) = {r}) ∧
+  (instr_assigns (Cxa_begin_catch r _) = {r}) ∧
+  (instr_assigns (Cxa_get_exception_ptr r _) = {r}) ∧
+  (instr_assigns _ = {})
+End
+
+Definition phi_assigns_def:
+  phi_assigns (Phi r _ _) = {r}
+End
+
+Inductive assigns:
+ (∀prog ip i r.
+    get_instr prog ip (Inl i) ∧
+    r ∈ instr_assigns i
+    ⇒
+    assigns prog ip r) ∧
+ (∀prog ip from_l phis r.
+    get_instr prog ip (Inr (from_l, phis)) ∧
+    r ∈ BIGUNION (set (map phi_assigns phis))
+    ⇒
+    assigns prog ip r)
 End
 
 Definition live_def:
-  live prog ip ⇔
-    { r | ∃path instr.
+  live prog ip =
+    { r | ∃path.
             good_path prog (ip::path) ∧
-            get_instr prog (last (ip::path)) instr ∧
-            r ∈ uses instr ∧
-            ∀ip2 instr2. ip2 ∈ set (front (ip::path)) ∧ get_instr prog ip2 instr2 ⇒ r ∉ assigns instr2 }
+            r ∈ uses prog (last (ip::path)) ∧
+            ∀ip2. ip2 ∈ set (front (ip::path)) ⇒ r ∉ assigns prog ip2 }
 End
 
+(*
 Theorem get_instr_live:
   ∀prog ip instr.
     get_instr prog ip instr
@@ -140,6 +188,7 @@ Proof
   qexists_tac `[]` >> rw [Once good_path_cases] >>
   qexists_tac `instr` >> simp [] >> metis_tac [IN_DEF]
 QED
+*)
 
 Triviality set_rw:
   !s P. (!x. x ∈ s ⇔ P x) ⇔ s = P
@@ -148,28 +197,24 @@ Proof
 QED
 
 Theorem live_gen_kill:
-  ∀prog ip instr ip'.
-    get_instr prog ip instr
-    ⇒
-    live prog ip = BIGUNION {live prog ip' | ip' ∈ next_ips instr ip} DIFF assigns instr ∪ uses instr
+  ∀prog ip ip'.
+    live prog ip =
+    BIGUNION {live prog ip' | ip' | ip' ∈ next_ips prog ip} DIFF assigns prog ip ∪ uses prog ip
 Proof
   rw [live_def, EXTENSION] >> eq_tac >> rw []
   >- (
-    Cases_on `path` >> fs []
-    >- metis_tac [get_instr_func] >>
+    Cases_on `path` >> fs [] >>
     rename1 `ip::ip2::path` >>
     qpat_x_assum `good_path _ _` mp_tac >> simp [Once good_path_cases] >> rw [] >>
-    Cases_on `x ∈ uses instr` >> fs [] >> simp [set_rw, PULL_EXISTS] >>
-    qexists_tac `ip2` >> qexists_tac `path` >> qexists_tac `instr'` >> rw [] >>
-    metis_tac [get_instr_func])
+    Cases_on `x ∈ uses prog ip` >> fs [] >> simp [set_rw, PULL_EXISTS] >>
+    qexists_tac `ip2` >> qexists_tac `path` >> rw [])
   >- (
     fs [] >>
-    qexists_tac `ip'::path` >> qexists_tac `instr'` >> rw []
-    >- (simp [Once good_path_cases] >> metis_tac []) >>
-    metis_tac [get_instr_func])
+    qexists_tac `ip'::path` >> rw [] >>
+    simp [Once good_path_cases])
   >- (
-    qexists_tac `[]` >> qexists_tac `instr` >> rw [] >>
-    simp [Once good_path_cases] >>
+    qexists_tac `[]` >> rw [] >>
+    fs [Once good_path_cases, uses_cases, IN_DEF] >>
     metis_tac [])
 QED
 
